Valid, isEmpty, isFull created

lab2/lab2.dfy
@@ -1,42 +1,73 @@
 // class CircularMemory
 // This class implements a circular buffer with 2 int typed pointers
 class CircularMemory
-{
+  {
   var cells : array<int>
   var read_position : int
   var write_position : int
   var isFlipped : bool
 
   constructor Init(cap : int)
-  //missing some pre-conditions here
-  requires cap > 0 
-  ensures Valid()
-  ensures fresh(cells)
-  ensures read_position == 0
-  ensures write_position == 0
-  ensures isFlipped == false
+    //missing some pre-conditions here
+    requires cap > 0
+    ensures read_position == 0
+    ensures write_position == 0
+    ensures isFlipped == false
+    ensures fresh(cells)
+    ensures isEmpty()
+    ensures Valid()
   {
     cells := new int[cap];
     read_position, write_position := 0, 0;
     isFlipped := false;
   }
-  
+
   // Valid is the class invariant we would like to maintain
   // for any CircularMemory at any moment of its lifetime
   predicate Valid()
-    reads this, this`cells
+    reads this//, this`cells, this`write_position, this`read_position // can still read fields?
   {
-  // Think of some constraints on: 
-  // 1. cells.Length?
-  // 2. write_position?
-  // 3. read_position?
-    HasElem(cells)
+    // Think of some constraints on:
+    // 1. cells.Length?
+    // 2. write_position?
+    // 3. read_position?
+    HasElem(cells) && WithinLimits(write_position) && WithinLimits(read_position)
   }
 
 
 
+  // A predicate indicating no more Read available
+  predicate isEmpty()
+    reads this
+  {
+    EqPointers() && !isFlipped
+  }
 
-  predicate HasElem(a : array) {
+
+  //A predicate indicating no more Write should be allowed
+  predicate isFull()
+    reads this
+  {
+    EqPointers() && isFlipped
+
+  }
+
+
+
+  predicate EqPointers() 
+  reads this`read_position, this`write_position
+  {
+    read_position == write_position
+  }
+
+  predicate HasElem(a : array)
+  {
     a.Length > 0
+  }
+
+  predicate WithinLimits(index : int)
+    reads this`cells
+  {
+    0 <= index && index < cells.Length
   }
 }
